Merge skyscraper + merkle examples

Examples/Merkle/Merkle/Ref.lean
@@ -1,5 +1,69 @@
-import Lampe
+import Merkle.Field
 
+open Merkle
 namespace Ref
 
-open Lampe
+open Lampe (U)
+
+def RC : Array bnField := #[
+    17829420340877239108687448009732280677191990375576158938221412342251481978692,
+    5852100059362614845584985098022261541909346143980691326489891671321030921585,
+    17048088173265532689680903955395019356591870902241717143279822196003888806966,
+    71577923540621522166602308362662170286605786204339342029375621502658138039,
+    1630526119629192105940988602003704216811347521589219909349181656165466494167,
+    7807402158218786806372091124904574238561123446618083586948014838053032654983,
+    13329560971460034925899588938593812685746818331549554971040309989641523590611,
+    16971509144034029782226530622087626979814683266929655790026304723118124142299
+]
+
+def SIGMA : bnField := 9915499612839321149637521777990102151350674507940716049588462388200839649614
+
+def rl (u : U 8) : U 8 :=
+    let top_bit := u >>> 7;
+    (u <<< 1) ||| top_bit
+
+def rotateLeft (u N : U 8) : U 8 := Nat.repeat rl N.toNat u
+
+def sbox (v : U 8) : U 8 :=
+  v ^^^ rotateLeft (rotateLeft v.not 1 &&& rotateLeft v 2 &&& rotateLeft v 3) 1
+
+def bar (a : bnField) : bnField :=
+  let bytes := a.toLeBytes
+  let left := bytes.take 16
+  let right := bytes.drop 16
+  let new_left := left.map sbox
+  let new_right := right.map sbox
+  let new_bytes := new_right.append new_left
+  bnField.fromLeBytes new_bytes
+
+def square (a : bnField) : bnField :=
+  a * a * SIGMA
+
+structure State where
+  left : bnField
+  right : bnField
+deriving Repr
+
+namespace State
+
+def permute (s : State) : State :=
+  let (l, r) := (s.left, s.right)
+  let (l, r) := (r + square l, l)
+  let (l, r) := (r + square l + RC[0], l)
+  let (l, r) := (r + bar l + RC[1], l)
+  let (l, r) := (r + bar l + RC[2], l)
+  let (l, r) := (r + square l + RC[3], l)
+  let (l, r) := (r + square l + RC[4], l)
+  let (l, r) := (r + bar l + RC[5], l)
+  let (l, r) := (r + bar l + RC[6], l)
+  let (l, r) := (r + square l + RC[7], l)
+  let (l, r) := (r + square l, l)
+  { left := l, right := r }
+
+def compress (v : List.Vector bnField 2) : bnField :=
+  let x := permute ⟨v[0], v[1]⟩
+  x.left + v[0]
+
+end State
+
+end Ref
