Examples/Merkle/Merkle/Spec.lean
@@ -1,4 +1,5 @@
 import Merkle.Extracted
+import Merkle.Field
 import Merkle.Ref
 import Lampe
 
@@ -6,13 +7,9 @@ import ProvenZk
 
 import Mathlib.Data.Vector.Snoc
 
-open Lampe Ref
+open Lampe Ref Extracted
 
-namespace Extracted
-
-def p := 21888242871839275222246405745257275088548364400416034343698204186575808495617 - 1
-
-axiom pPrime : Nat.Prime (p + 1)
+namespace Spec
 
 def lp : Lampe.Prime := ⟨p, pPrime⟩
 
@@ -103,30 +100,331 @@ theorem recover_intro {H N idx proof item}
   congr
   all_goals simp
 
-instance {α H n} : Membership α (MerkleTree α H n) where
-  mem t e := ∃p, e = MerkleTree.itemAt t p
+def RC : List Int :=
+    [-4058822530962036113558957735524994411356374024839875405476791844324326516925,
+    5852100059362614845584985098022261541909346143980691326489891671321030921585,
+    -4840154698573742532565501789862255731956493498174317200418381990571919688651,
+    71577923540621522166602308362662170286605786204339342029375621502658138039,
+    1630526119629192105940988602003704216811347521589219909349181656165466494167,
+    7807402158218786806372091124904574238561123446618083586948014838053032654983,
+    -8558681900379240296346816806663462402801546068866479372657894196934284905006,
+    -4916733727805245440019875123169648108733681133486378553671899463457684353318]
 
-def DH : Hash (Fp lp) 2 := fun vec![a, b] => a + b
+def SIGMA : Int :=
+    9915499612839321149637521777990102151350674507940716049588462388200839649614
 
-lemma DummyHash_correct:
-    STHoare lp env
-        ⟦True⟧
-        (Expr.call [Tp.field, Tp.field] Tp.field
-          (FuncRef.trait (some $ «struct#DummyHasher».tp h![]) "BinaryHasher" [Kind.type] (HList.cons Tp.field HList.nil) "hash" [] HList.nil) h![a,b])
-        (fun v => v = DH vec![a,b]) := by
-  enter_trait [] env
+theorem rl_intro : STHoare lp env ⟦⟧
+  (Expr.call [Tp.u 8] (Tp.u 8) (FuncRef.decl "rl" [] HList.nil) h![input])
+    fun output => output = Ref.rl input := by
+  enter_decl
   steps
   subst_vars
   rfl
 
-theorem main_correct [Fact (CollisionResistant DH)] {tree : MerkleTree (Fp lp) DH 32}:
+theorem u8_ge_zero (u : U 8) : 0 ≤ u := by bv_decide
+
+theorem rotateLeft_spec : STHoare lp env ⟦N < 254⟧ (rotate_left.fn.body _ h![] |>.body h![input, N])
+    fun output => output = Ref.rotateLeft input N := by
+  simp only [Extracted.rotate_left]
+
+  steps
+  loop_inv fun i _ _ => [result ↦ ⟨Tp.u 8, Nat.repeat Ref.rl i.toNat input⟩]
+  change 0 ≤ N
+  exact u8_ge_zero N
+  · intros i hlo hhi
+    steps [rl_intro]
+    simp_all
+    congr
+    have : (i.toNat + 1) % 256 = i.toNat + 1 := by
+      have : i.toNat < N.toNat := hhi
+      have : N.toNat < 254 := by rename_i a _ _ ; exact a
+      omega
+    rw [this]
+    simp [Nat.repeat]
+  · steps
+    simp_all [Ref.rotateLeft]
+
+theorem rotate_left_intro : STHoare lp env ⟦N < 254⟧
+    (Expr.call [Tp.u 8, Tp.u 8] (Tp.u 8) (FuncRef.decl "rotate_left" [] HList.nil) h![input, N])
+      fun output => output = Ref.rotateLeft input N := by
+  enter_decl
+  apply STHoare.consequence (h_hoare := rotateLeft_spec)
+  simp_all [SLP.entails]
+  simp [SLP.star, SLP.top, SLP.entails]
+
+theorem sbox_spec : STHoare lp env ⟦⟧ (sbox.fn.body _ h![] |>.body h![input])
+    fun output => output = Ref.sbox input := by
+  simp only [Extracted.sbox]
+  steps [rotate_left_intro]
+  · subst_vars; rfl
+  all_goals decide
+
+theorem sbox_intro : STHoare lp env ⟦⟧ (Expr.call [Tp.u 8] (Tp.u 8) (FuncRef.decl "sbox" [] HList.nil) h![input])
+    fun output => output = Ref.sbox input := by
+  enter_decl
+  apply sbox_spec
+
+theorem sgn0_spec : STHoare lp env ⟦⟧ (Expr.call [Tp.field] (Tp.u 1) (FuncRef.decl "sgn0" [] HList.nil) h![input])
+    fun output => output = (input.val % 2) := by
+  enter_decl
+  simp only [sgn0]
+  steps
+  simp_all
+
+opaque BitVec.bytesLE : BitVec n → List.Vector (U 8) n
+
+axiom toLeBytesPadLen {input : Lampe.Fp lp} : (padEnd 32 (Lampe.toLeBytes input)).length = 32
+
+axiom to_le_bytes_intro {input} : STHoare lp env ⟦⟧ (Expr.call [Tp.field] (Tp.array (Tp.u 8) 32) (FuncRef.decl "to_le_bytes" [] HList.nil) h![input])
+    fun output => output = ⟨List.takeD 32 (Lampe.toLeBytes input) 0, List.takeD_length _ _ _⟩
+
+axiom from_le_bytes_intro {input} : STHoare lp env ⟦⟧ (Expr.call [Tp.array (Tp.u 8) 32] Tp.field (FuncRef.decl "from_le_bytes" [] HList.nil) h![input])
+    fun output => output = Merkle.bnField.fromLeBytes input.toList
+
+def _root_.List.Vector.pad {α n} (v : List.Vector α n) (d : Nat) (pad : α) : List.Vector α d := match d, n with
+| 0, _ => List.Vector.nil
+| d+1, 0 => pad ::ᵥ List.Vector.pad v d pad
+| d+1, _+1 => v.head ::ᵥ List.Vector.pad v.tail d pad
+
+@[simp]
+theorem List.Vector.toList_pad {v : List.Vector α n} {pad} : (v.pad d pad).toList = v.toList.takeD d pad := by
+  rcases v with ⟨l, prop⟩
+  induction d generalizing l n with
+  | zero => simp
+  | succ d ih =>
+    cases n
+    · simp [List.Vector.pad, ih, List.replicate_succ]
+    · rcases (List.exists_of_length_succ _ prop) with ⟨h, t, ⟨rfl⟩⟩
+      simp at prop
+      simp [List.Vector.pad, List.Vector.head, List.Vector.tail, ih]
+
+theorem List.takeD_eq_take_append : List.takeD n l pad = List.take n l ++ List.replicate (n - l.length) pad := by
+  induction n generalizing l with
+  | zero => simp
+  | succ n ih =>
+    cases l
+    · simp [List.replicate]
+    · simp [List.takeD, List.take, ih]
+
+theorem as_array_intro (hi : input.length = 32) : STHoare lp env ⟦⟧ (Expr.call [Tp.slice (Tp.u 8)] (Tp.array (Tp.u 8) 32) (FuncRef.decl "as_array" [] HList.nil) h![input])
+    fun output => output = ⟨input, hi⟩ := by
+  enter_decl
+  simp only [as_array]
+  steps
+  loop_inv fun i _ _ => [array ↦ ⟨Tp.array (Tp.u 8) 32, List.Vector.pad ⟨input.takeD i.toNat 0#8, List.takeD_length i.toNat _ _⟩ 32 0#8⟩]
+  · decide
+  · intros i hlo hhi
+    steps
+    casesm* ∃_,_
+    subst_vars
+    simp [Access.modify]
+    congr 1
+    rcases i with ⟨i, _⟩
+    simp [IntCast.intCast, Int.cast, Fin.lt_def, OfNat.ofNat] at hhi
+    apply List.Vector.eq
+    simp only [List.Vector.toList_set, List.Vector.toList_pad, BitVec.toNat]
+    simp only [List.Vector.toList]
+    rw [Nat.mod_eq_of_lt (by linarith)]
+    simp only [List.takeD_eq_take_append]
+    have : i ≤ 32 := by linarith
+    have : i + 1 ≤ 32 := by linarith
+    simp [*, List.take_take]
+    rw [List.take_succ, List.append_assoc]
+    congr 1
+    generalize_proofs
+    have : 32 - i = (31 - i) + 1 := by omega
+    simp [getElem?, decidableGetElem?, *, List.replicate]
+  steps
+  subst_vars
+  apply List.Vector.eq
+  simp only [List.Vector.toList_pad]
+  simp only [List.Vector.toList]
+  conv => enter [1,2,1]; whnf
+  have : input.length ≤ input.length := by linarith
+  simp only [←hi, Int.cast, IntCast.intCast, BitVec.ofInt, List.takeD_eq_take, this, List.take_length]
+
+set_option maxHeartbeats 3000000000000
+theorem bar_spec : STHoare lp env ⟦⟧ (bar.fn.body _ h![] |>.body h![input])
+    fun output => output = Ref.bar input := by
+  simp only [Extracted.bar]
+  steps [to_le_bytes_intro]
+
+  enter_block_as
+    ([new_left ↦ ⟨(Tp.u 8).array 16, List.Vector.replicate 16 0⟩])
+    (fun _ => [new_left ↦ ⟨(Tp.u 8).array 16, bytes.take 16 |>.map Ref.sbox⟩])
+
+  · loop_inv fun i _ _ => [new_left ↦ ⟨(Tp.u 8).array 16, bytes.take i.toNat |>.map Ref.sbox |>.pad 16 (0:U 8)⟩]
+    · decide
+    · congr 1
+      apply List.Vector.eq
+      simp [-List.takeD_succ, List.takeD_eq_take_append, Int.cast, IntCast.intCast]
+    · intro i _ hlt
+      rename bytes = _ => bytes_def
+      clear bytes_def
+      steps [sbox_intro]
+      rcases i with ⟨i, hi⟩
+      rw [BitVec.lt_def] at hlt
+      conv at hlt => congr <;> whnf
+      have : i + 1 < 4294967296 := by
+        linarith
+      casesm* ∃_,_
+      subst_vars
+      congr 1
+      apply List.Vector.eq
+      simp [-List.takeD_zero, -List.takeD_succ, Access.modify, List.Vector.get, Fin.add_def, Nat.mod_eq_of_lt, this]
+      have i₁ : i ≤ 32 := by linarith
+      have i₂ : i + 1 ≤ 32 := by linarith
+      have i₃ : i ≤ 16 := by linarith
+      have i₄ : i + 1 ≤ 16 := by linarith
+      have i₅ : i < 32 := by linarith
+      simp [-List.takeD_zero, -List.takeD_succ,
+        List.takeD_eq_take_append,
+        List.take_take,
+        i₁, i₂, i₃, i₄]
+      simp only [List.take_succ, List.append_assoc]
+      have : (16 - i) = (15 - i) + 1 := by omega
+      simp [this, List.replicate_succ, getElem?, decidableGetElem?, i₅, List.Vector.toList]
+
+  steps
+
+  enter_block_as
+    ([new_right ↦ ⟨(Tp.u 8).array 16, List.Vector.replicate 16 0⟩])
+    (fun _ => [new_right ↦ ⟨(Tp.u 8).array 16, bytes.drop 16 |>.map Ref.sbox⟩])
+
+  · loop_inv fun i _ _ => [new_right ↦ ⟨(Tp.u 8).array 16, bytes.drop 16 |>.take i.toNat |>.map Ref.sbox |>.pad 16 (0:U 8)⟩]
+    · decide
+    · congr 1
+      apply List.Vector.eq
+      simp [-List.takeD_succ, Int.cast, IntCast.intCast, List.takeD_eq_take_append, List.take_take]
+    · intro i _ hlt
+      rename bytes = _ => bytes_def
+      clear bytes_def
+      steps [sbox_intro]
+      casesm* ∃_,_
+      subst_vars
+      rcases i with ⟨i, hi⟩
+      rw [BitVec.lt_def] at hlt
+      conv at hlt => congr <;> whnf
+      simp [-List.takeD_zero, -List.takeD_succ, Builtin.CastTp.cast, Access.modify]
+      congr 1
+      apply List.Vector.eq
+      simp [-List.takeD_zero, -List.takeD_succ, -List.map_drop, List.Vector.get, Fin.add_def, Int.cast, IntCast.intCast, OfNat.ofNat]
+      have : 16 + i < 4294967296 := by linarith
+      have : i + 1 < 4294967296 := by linarith
+      simp only [Nat.mod_eq_of_lt, *, List.getElem_drop']
+      simp only [List.takeD_eq_take_append]
+      have i₁ : i ≤ 16 := by linarith
+      have i₂ : i + 1 ≤ 16 := by linarith
+      simp [i₁, i₂, List.take_take]
+      simp only [List.take_succ, List.append_assoc]
+      congr 1
+      have : (16 - i) = (15 - i) + 1 := by omega
+      simp [this, List.replicate_succ, getElem?, decidableGetElem?]
+      simp only [hlt, dite_true, Option.toList]
+      simp [List.cons_append, List.nil_append, List.Vector.toList]
+
+  steps
+
+  rename' «#v_25» => v
+
+  enter_block_as =>
+    ([new_bytes ↦ ⟨(Tp.u 8).slice, v.toList⟩])
+    (fun _ => [new_bytes ↦ ⟨(Tp.u 8).slice, v.toList ++ ζi0.toList⟩])
+  · loop_inv fun i _ _ => [new_bytes ↦ ⟨(Tp.u 8).slice, v.toList ++ ζi0.toList.take i.toNat⟩]
+    · decide
+    · congr 1
+      simp [Int.cast, IntCast.intCast]
+    · congr 1
+      simp
+    · intro i _ hlt
+      rename bytes = _ => bytes_def
+      clear bytes_def
+      steps
+      simp
+      congr 1
+      rcases i with ⟨i, hi⟩
+      rw [BitVec.lt_def] at hlt
+      conv at hlt => congr <;> whnf
+      casesm* ∃_,_
+      subst «#v_30» elem
+      have : i + 1 < 4294967296 := by linarith
+      simp [Nat.mod_eq_of_lt, this, List.take_succ]
+      simp [getElem?, decidableGetElem?, hlt]
+      rfl
+
+  steps [as_array_intro, from_le_bytes_intro]
+  rotate_left
+  · subst «#v_35» v
+    simp
+  · subst_vars
+    rfl
+
+theorem bar_intro : STHoare lp env ⟦⟧ (Expr.call [Tp.field] Tp.field (FuncRef.decl "bar" [] HList.nil) h![input])
+    fun output => output = Ref.bar input := by
+  enter_decl
+  apply bar_spec
+
+theorem sigma_intro : STHoare lp env (⟦⟧)
+    (Expr.call [] Tp.field (FuncRef.decl "SIGMA" [] HList.nil) h![])
+      fun output => output = Ref.SIGMA := by
+  enter_decl
+  simp only [Extracted.SIGMA]
+  steps []
+  unfold Ref.SIGMA
+  assumption
+
+theorem rc_intro : STHoare lp env (⟦⟧)
+    (Expr.call [] (Tp.field.array 8) (FuncRef.decl "RC" [] HList.nil) h![])
+      fun output => output = ⟨Ref.RC.toList, by rfl⟩ := by
+  enter_decl
+  simp only [Extracted.RC]
+  steps []
+  subst_vars
+  unfold Ref.RC
+  rfl
+
+theorem square_intro : STHoare lp env (⟦⟧)
+    (Expr.call [Tp.field] Tp.field (FuncRef.decl "square" [] HList.nil) h![input])
+      fun output => output = Ref.square input := by
+  enter_decl
+  simp only [Extracted.square]
+  steps [sigma_intro]
+  unfold Ref.square
+  subst_vars
+  rfl
+
+theorem permute_intro : STHoare lp env ⟦⟧ (Expr.call [Tp.field.array 2] (Tp.field.array 2) (FuncRef.decl "permute" [] HList.nil) h![i])
+    fun output => output = (Ref.State.permute ⟨i[0], i[1]⟩).1 ::ᵥ (Ref.State.permute ⟨i[0], i[1]⟩).2 ::ᵥ List.Vector.nil := by
+  enter_decl
+  cases i using List.Vector.casesOn with | cons _ i =>
+  cases i using List.Vector.casesOn with | cons _ i =>
+  cases i using List.Vector.casesOn
+  simp only [Extracted.permute]
+  steps [bar_intro, square_intro, rc_intro]
+  casesm* ∃_,_
+  simp [Builtin.indexTpl, Nat.mod_eq_of_lt, lp] at *
+  subst_vars
+  rfl
+
+instance {α H n} : Membership α (MerkleTree α H n) where
+  mem t e := ∃p, e = MerkleTree.itemAt t p
+
+lemma SkyscraperHash_correct: STHoare lp env ⟦⟧ (Expr.call [Tp.field, Tp.field] Tp.field
+          (FuncRef.trait (some $ «struct#Skyscraper».tp h![]) "BinaryHasher" [Kind.type] (HList.cons Tp.field HList.nil) "hash" [] HList.nil) h![a,b]) (fun v => v = Ref.State.compress ⟨[a, b], rfl⟩) := by
+  enter_trait [] env
+  steps [permute_intro]
+  casesm*∃_,_
+  subst_vars
+  congr 1
+
+theorem main_correct [Fact (CollisionResistant Ref.State.compress)] {tree : MerkleTree (Fp lp) Ref.State.compress 4}:
     STHoare lp env
         ⟦⟧
         (main.call h![] h![tree.root, proof, item, index])
         (fun _ => item ∈ tree) := by
   enter_decl
   simp only
-  steps [recover_intro (H:= «struct#DummyHasher».tp h![]) (N:=32) (hHash := DummyHash_correct)]
+  steps [recover_intro (H:= «struct#Skyscraper».tp h![]) (N:=4) (hHash := SkyscraperHash_correct)]
   use index.reverse
   rename ∃_, True => heq
   simp at heq
