Examples/Skyscraper/Skyscraper.lean
@@ -1,4 +1,0 @@
-import Skyscraper.Extracted
-import Skyscraper.Field
-import Skyscraper.Ref
-import Skyscraper.Spec
